iris/WeakRobustTrace.v
@@ -338,22 +338,23 @@ Section trace.
   Lemma astep_ok_ts_none img log i (ag : wpagent P) l f Dl :
     astep_ok img log i ag l f Dl →
     match l with
-    | LStore _ _ _ _ _ | LRmw _ _ _ _ _ _ _ => True
+    | LStore _ _ _ _ _ | LRmw _ _ _ _ _ _ _ | LExStore _ _ _ _ _ => True
     | LSilent | LLoad _ _ _ _ _ | LFence _ _ _ _ | LDev | LRegW _ _
-    | LCtrl _ | LInstr => Dl = None
+    | LCtrl _ | LInstr | LExLoad _ _ _ _ => Dl = None
     end.
   Proof.
     destruct l; simpl;
       [by intros [_ ->]|by intros (_ & _ & ->)|done|done|by intros [_ ->]
-      |by intros [_ ->]|by intros [_ ->]|by intros [_ ->]|by intros [_ ->]].
+      |by intros [_ ->]|by intros [_ ->]|by intros [_ ->]|by intros [_ ->]
+      |done|done].
   Qed.
 
   Lemma atrace_ts_none img log i T k ev :
     atrace_wf img log i T → at_evs T !! k = Some ev →
     match ae_lb ev with
-    | LStore _ _ _ _ _ | LRmw _ _ _ _ _ _ _ => True
+    | LStore _ _ _ _ _ | LRmw _ _ _ _ _ _ _ | LExStore _ _ _ _ _ => True
     | LSilent | LLoad _ _ _ _ _ | LFence _ _ _ _ | LDev | LRegW _ _
-    | LCtrl _ | LInstr => ae_ts ev = None
+    | LCtrl _ | LInstr | LExLoad _ _ _ _ => ae_ts ev = None
     end.
   Proof.
     intros Hwf Hev.
@@ -373,8 +374,8 @@ Section trace.
     destruct (asteps_wf_step _ _ _ _ _ _ _ Hwf Hev)
       as (ag & ag' & st' & f & _ & _ & Hps & _ & _).
     apply (astep_prog_step d0) in Hps as (d & d' & Hps).
-    destruct (ae_lb ev) as [|aq lat base tvs asrc| | | | | | |]; simpl;
-      [done| |done|done|done|done|done|done|done].
+    destruct (ae_lb ev) as [|aq lat base tvs asrc| | | | | | | | |]; simpl;
+      [done| |done|done|done|done|done|done|done|done|done].
     destruct lat; [|done]. by destruct (Hlfp _ _ _ _ _ _ _ _ Hps).
   Qed.
 
